src/verification/stream_zero.lean
@@ -1,0 +1,25 @@
+import verification.stream
+
+variables {ι : Type} {α β : Type*}
+
+@[simps]
+instance [has_zero β] : has_zero (Stream ι β) :=
+⟨{ σ := unit,
+  valid := λ _, false,
+  ready := λ _, false,
+  next := λ _, false.elim,
+  index := λ _, false.elim,
+  value := λ _, false.elim }⟩
+
+@[simp] lemma Stream.zero_eval [add_zero_class β] (n : ℕ) (x : unit) :
+  (0 : Stream ι β).eval_steps n x = 0 := Stream.eval_invalid not_false _
+
+@[simps]
+instance [has_zero β] : has_zero (StreamExec ι β) := ⟨
+{ stream := 0,
+  state := (),
+  bound := 0 }⟩
+
+@[simp] lemma StreamExec.zero_eval [add_zero_class β] :
+  (0 : StreamExec ι β).eval = 0 := rfl
+
